Definitions/Regions.v
@@ -8,9 +8,9 @@ Definition RgnId :=  nat.
 Definition VarId := ascii.
 
 Inductive Region : bool * bool * bool -> Set :=
-  | Rgn2_Const : forall fv bv, RgnId -> Region (true, fv, bv)
-  | Rgn2_FVar : forall c bv, VarId -> Region (c, true, bv)
-  | Rgn2_BVar : forall c fv, nat -> Region (c, fv, true).
+  | Rgn_Const : forall fv bv, RgnId -> Region (true, fv, bv)
+  | Rgn_FVar : forall c bv, VarId -> Region (c, true, bv)
+  | Rgn_BVar : forall c fv, nat -> Region (c, fv, true).
 Definition Region_in_Expr := Region (true, true, false).
 Definition Region_in_Type := Region (true, true, true).
 
@@ -24,9 +24,9 @@ Definition Rho := R.t RgnId.
 
 Definition find_R (k: Region_in_Expr) (m: Rho) : option RgnId :=
  match k with 
-  | Rgn2_Const fv bv n => Some n
-  | Rgn2_FVar c bv n => R.find (elt := RgnId) n m
-  | Rgn2_BVar c fv n => None                               
+  | Rgn_Const fv bv n => Some n
+  | Rgn_FVar c bv n => R.find (elt := RgnId) n m
+  | Rgn_BVar c fv n => None                               
  end.
 
 Definition update_R (p: VarId * RgnId) (m : Rho) := R.add (fst p) (snd p) m.
