Definitions/StaticActions.v
@@ -3,17 +3,13 @@ Require Import Definitions.Regions.
 
 (* Static Actions; for type-and-effect system *)
 Inductive StaticAction : Set :=
-| SA2_Alloc : Region_in_Type -> StaticAction
-| SA2_Read  : Region_in_Type -> StaticAction
-| SA2_Write : Region_in_Type -> StaticAction.
+| SA_Alloc : Region_in_Type -> StaticAction
+| SA_Read  : Region_in_Type -> StaticAction
+| SA_Write : Region_in_Type -> StaticAction.
 
 Definition Epsilon := Ensemble StaticAction.
 
 (* Static Actions; for type-and-effect system *)
-Definition SA_Alloc:= SA2_Alloc.
-Definition SA_Read:= SA2_Read.
-Definition SA_Write:= SA2_Write.
-
 Definition Empty_Static_Action := Empty_set StaticAction.
 Definition Singleton_Static_Action (e : StaticAction) :=  Singleton StaticAction e.
 Definition Union_Static_Action (a b : Ensemble StaticAction) :=  Union StaticAction a b.
@@ -30,7 +26,7 @@ Inductive ReadOnlyStatic : Epsilon -> Prop :=
 
 
 Inductive Disjoint_Static : StaticAction -> StaticAction -> Prop :=
- | DS_Read_Read   : forall r1 r2, Disjoint_Static (SA2_Read r1) (SA2_Read r2)
- | DS_Write_Write : forall r1 r2, r1 <> r2 -> Disjoint_Static (SA2_Write r1) (SA2_Write r2)
- | DS_Read_Write  : forall r1 r2, r1 <> r2 -> Disjoint_Static (SA2_Read r1) (SA2_Write r2)
- | DS_Write_Read  : forall r1 r2, r1 <> r2 -> Disjoint_Static (SA2_Write r1) (SA2_Read r2).
+ | DS_Read_Read   : forall r1 r2, Disjoint_Static (SA_Read r1) (SA_Read r2)
+ | DS_Write_Write : forall r1 r2, r1 <> r2 -> Disjoint_Static (SA_Write r1) (SA_Write r2)
+ | DS_Read_Write  : forall r1 r2, r1 <> r2 -> Disjoint_Static (SA_Read r1) (SA_Write r2)
+ | DS_Write_Read  : forall r1 r2, r1 <> r2 -> Disjoint_Static (SA_Write r1) (SA_Read r2).
